src/proof/k8s_io/kubernetes/pkg/controller.v
@@ -1,0 +1,23 @@
+From New.proof Require Import prelude empty_ffi.
+From New.proof Require Export pure_objects.
+From New.proof.k8s_io.kubernetes.pkg Require Export controller_init.
+
+
+Section proof.
+Context `{hG: !heapGS Σ} {go_ctx: GoContext}.
+
+Lemma wp_PodControllerIndexKey namespace ownerReference owner_reference dq:
+  {{{ is_pkg_init controller ∗
+      ownerReference ↦{dq} owner_reference
+  }}}
+  @! controller.PodControllerIndexKey #namespace #ownerReference
+  {{{ index_key, RET #index_key;
+      ⌜ index_key =  namespace ++ "/"%go ++ 
+        owner_reference.(v1.OwnerReference.Kind') ++ "/"%go ++ 
+        owner_reference.(v1.OwnerReference.Name') ++ "/"%go ++
+        owner_reference.(v1.OwnerReference.UID')⌝
+  }}}.
+Proof.
+Admitted.
+
+End proof.
